\documentclass[12pt]{article}
\usepackage [margin=1in]{geometry}
\usepackage{amsmath, amssymb}

\begin{document}

Homework 2
Isaac Kim
Professor Snyder
CS 463
Feb 10, 2023

\iffalse
1.1 
	((λn.n-3)8)
==> E-App-Abs
	8-3
==> E-Sub
	5

1.2
	((λa.a+1)(2+3))
==> E-App2 via E-Add
	((λa.a+1)(5))
==> E-App-Abs
	5+1
==> E-Add
	6

1.3
	( ( (λx. (λy. if (x=y) x 0) ) (1+4)) (2*3))
==> E-App2 via E-Add
	( ( (λx. (λy. if (x=y) x 0) ) 5) (2*3))
==> E-App-Abs
	((λy. if (5=y) 5 0 ) (2*3))
==> E-App2 via E-Mul
	((λy. if (5=y) 5 0 ) (6))
==> E-App-Abs
	(if (5=6) 5 0 )
==> E-If
	(if false 5 0 )
==> E-If-False
	0

1.4
	(((λf. λn. (f n)) (λx.4*x)) 7)
==> E-App-Abs
	((λn. ((λx.4*x) n)) 7)
==> E-App-Abs
	((λx.4*x) 7)
==> E-App-Abs
	(4*7)
==> E-Mul
	28

1.5
	((λxs. cons 3 xs) (if true (cons 2 nil) nil))
==> E-App2 via E-If-True
	((λxs. cons 3 xs) (cons 2 nil))
==> E-App-Abs
	( cons 3 (cons 2 nil))

2.1
	(not false)
==> Expand not
	((λa. (a false) true) false)
==> E-App-Aps
	(false false) true) 
==> Expand false
	((λx. λy. y) false) true)
==> E-App1 via E-App-Abs
	(λy. y) true)
==> E-App-Abs
	true

2.2
((or true) false)
==> Expand OR
(((λa. λb. (a a) b) true) false)
==> E-App1 via E-App-Abs
(λb.(true true) b) false)
==> E-App-Abs
(true true) false
==> Expand true
((λx. λy. x) true) false
==> E-App1 via E-App-Abs
(λy. true) false
==> E-App-Abs
true

2.3
((and true) false)
==> Expand and
(((λa. λb. (a b) a) true) false)
==> E-App1 via E-App-Abs
((λb. (true b) true) false)
==> E-App-Abs
(true false) true)
==> Expand true
((λx. λy. x) false) true)
==> E-App-Abs
(λy. false) true)
==> E-App-Abs
false

2.4
nand = λa. λb. (a (not b)) not a

2.5
((nand true) false)
==> Expand nand
(((λa. λb. (a (not b)) not a) true) false)
==> E-App1 via E-App-Abs
((λb. (true (not b)) not true) false)
==> E-App-Abs
((true (not false)) not true)
==> Expand true
(((λx. λy. x) (not false)) not true)
==> E-App1 via E-App2 (via question 1.1)
(((λx. λy. x) true) not true)
==> E-App1 via E-App-Abs
((λy. true) not true)
==> Expand not
((λy. true) (λa. (a false) true) true)
==> E-App2 via E-App-Abs
((λy. true) (true false) true)
==> Expand true
((λy. true) ((λx. λy. x) false) true)
==> E-App2 via E-App-Abs
((λy. true) (λy. false) true)
==> E-App2 via E-App-Abs
((λy. true) false
==> E-App-Abs
true
\fi

\noindent \textbf{3.1} 

\noindent \textbf{a)} 

\noindent E-orelse1 = $\frac{t_1 \rightarrow t'_1}{\text{orelse }t_1 t_2\rightarrow \text{orelse }t'_1 t_2}$
\\
\\
E-orelse2 = $\frac{}{\text{orelse (optional \emph{t}) } t_2\rightarrow t}$
\\
\\
E-orelse3 = $\frac{}{\text{orelse (empty) } t_2\rightarrow t_2}$
\\
\\
\noindent \textbf{b)}

\noindent E-get1 = $\frac{t \rightarrow t'}{\text{get }t\rightarrow \text{get }t'}$
\\
\\
E-get2 = $\frac{}{\text{get (optional \emph{t})}\rightarrow t}$
\\
\\
\noindent \textbf{c)}

\noindent E-ispresent1 = $\frac{t \rightarrow t'}{\text{ispresent }t\rightarrow \text{ispresent }t'}$
\\
\\
E-ispresent2 = $\frac{}{\text{ispresent (optional \emph{t})}\rightarrow \text{true}}$
\\
\\
E-ispresent3 = $\frac{}{\text{ispresent (empty)}\rightarrow \text{false}}$
\\
\\
\noindent \textbf{3.2} 

\noindent more = $\lambda a.\lambda b.(a+$(orelse \emph{b} 0))
\\
\\
isbig = $\lambda x.$ (if ispresent x (if $(x > 1000)$ optional true optional false) empty)
\end{document}
